wip

src/sequential/SequentialDef.v
@@ -20,14 +20,129 @@ Module Perm.
   | none
   | full
   .
-End Perm.
 
-Definition Perms := Loc.t -> Perm.t.
+  Definition le (p0 p1: t): bool :=
+    match p0, p1 with
+    | none, _ => true
+    | _, full => true
+    | _, _ => false
+    end.
+End Perm.
 Definition flag := bool.
 
-Definition SMemory := Loc.t -> Const.t * flag.
+Module SeqMemory.
+  Definition t := Loc.t -> Const.t * flag.
 
-Definition Oracle: Type. Admitted.
+  Definition update (loc: Loc.t) (val: Const.t) (m: t): t :=
+    fun loc' => if Loc.eq_dec loc' loc then (val, true) else (m loc').
+End SeqMemory.
+
+
+
+Variant diff :=
+| diff_rlx
+| diff_rel (val: Const.t) (f: flag)
+| diff_acq (val: Const.t)
+| diff_relacq (valw: Const.t) (f: flag) (valr: Const.t)
+.
+
+Definition diffs := Loc.t -> diff.
+
+Definition is_acq (d: diff): bool :=
+  match d with
+  | diff_acq _  => true
+  | _ => false
+  end.
+
+Definition is_rel (d: diff): bool :=
+  match d with
+  | diff_rel _ _  => true
+  | _ => false
+  end.
+
+Definition is_rlx (d: diff): bool :=
+  match d with
+  | diff_rlx => true
+  | _ => false
+  end.
+
+Variant wf_diff (d: diffs): forall (e: ProgramEvent.t), Prop :=
+| wf_diff_syscall
+    e
+  :
+    wf_diff d (ProgramEvent.syscall e)
+| wf_diff_fence
+    ordr ordw
+    (ACQ: forall loc (ORD: is_acq (d loc)), Ordering.le Ordering.acqrel ordr)
+    (REL: forall loc (ORD: is_rel (d loc)), Ordering.le Ordering.acqrel ordw)
+  :
+    wf_diff d (ProgramEvent.fence ordr ordw)
+| wf_diff_read
+    loc val ord
+    (REL: forall loc' (NEQ: loc' <> loc) (ORD: is_rel (d loc)), False)
+    (ACQ: forall loc' (NEQ: loc' <> loc) (ORD: is_acq (d loc)),
+        Ordering.le Ordering.acqrel ord)
+    (NA: Ordering.le Ordering.plain ord)
+  :
+    wf_diff d (ProgramEvent.read loc val ord)
+| wf_diff_write
+    loc val ord
+    (ACQ: forall loc' (NEQ: loc' <> loc) (ORD: is_acq (d loc)), False)
+    (REL: forall loc' (NEQ: loc' <> loc) (ORD: is_rel (d loc)),
+        Ordering.le Ordering.acqrel ord)
+    (NA: Ordering.le Ordering.plain ord)
+  :
+    wf_diff d (ProgramEvent.write loc val ord)
+| wf_diff_update
+    loc valr valw ordr ordw
+    (ACQ: forall loc' (NEQ: loc' <> loc) (ORD: is_acq (d loc)),
+        Ordering.le Ordering.acqrel ordr)
+    (REL: forall loc' (NEQ: loc' <> loc) (ORD: is_rel (d loc)),
+        Ordering.le Ordering.acqrel ordw)
+    (ORDR: Ordering.le Ordering.plain ordr)
+    (ORDW: Ordering.le Ordering.plain ordw)
+  :
+    wf_diff d (ProgramEvent.update loc valr valw ordr ordw)
+.
+
+Definition Perms := Loc.t -> Perm.t.
+
+
+Module Oracle.
+  Definition t: Type. Admitted.
+
+  Definition step:
+    forall (e: ProgramEvent.t)
+           (d: diffs)
+           (o0: t)
+           (o1: t), Prop.
+  Admitted.
+
+  Lemma step_wf e d o0 o1
+        (STEP: step e d o0 o1)
+    :
+      wf_diff d e.
+  Admitted.
+End Oracle.
+
+
+
+Definition
+
+
+Module SeqLocal.
+  Variant step:
+    forall (e: ProgramEvent.t)
+           (m0: SeqMemory.t) (p0: Perms) (o0: Oracle)
+           (m1: SeqMemory.t) (p1: Perms) (o1: Oracle), Prop :=
+  .
+End SeqLocal.
+
+
+
+De
+
+
 
 Module State.
 Section LANG.
@@ -36,18 +151,168 @@ Section LANG.
   Record t :=
     mk {
         state: lang.(Language.state);
-        memory: SMemory;
+        memory: SeqMemory.t;
         perm: Perms;
         oracle: Oracle;
       }.
 
-  Variant na_step: t -> t -> Prop :=
-  | na_step_silent
+  (* without oracle *)
+  Variant na_local_step (p: Perms) (o: Oracle):
+    forall (e: MachineEvent.t)
+           (pe: ProgramEvent.t)
+           (m0: SeqMemory.t)
+           (m1: SeqMemory.t), Prop :=
+  | na_local_step_silent
+      m
+    :
+      na_local_step
+        p o
+        (MachineEvent.silent) (ProgramEvent.silent)
+        m m
+  | na_local_step_read
+      m
+      loc val ord
+      (ORD: Ordering.le ord Ordering.na)
+      (VAL: Perm.le Perm.full (p loc) -> fst (m loc) = val)
+    :
+      na_local_step
+        p o
+        (MachineEvent.silent) (ProgramEvent.read loc val ord)
+        m m
+  | na_local_step_write
+      m0 m1 e
+      loc val ord
+      (ORD: Ordering.le ord Ordering.na)
+      (MEM: SeqMemory.update loc val m0 = m1)
+      (PERM: e = if Perm.le Perm.full (p loc) then MachineEvent.silent else MachineEvent.failure)
+    :
+      na_local_step
+        p o
+        e (ProgramEvent.write loc val ord)
+        m0 m1
+  | na_local_step_failure
+      m
+    :
+      na_local_step
+        p o
+        (MachineEvent.failure) (ProgramEvent.failure)
+        m m
+  | na_local_step_update
+      m
+      loc valr valw ordr ordw
+      (ORD: __guard__(Ordering.le ordr Ordering.na \/ Ordering.le ordw Ordering.na))
+    :
+      na_local_step
+        p o
+        (MachineEvent.failure) (ProgramEvent.update loc valr valw ordr ordw)
+        m m
+  .
+
+  Variant na_step: MachineEvent.t -> t -> t -> Prop :=
+  | na_step_intro
+      p o
+      st0 st1 m0 m1 e pe
+      (LANG: lang.(Language.step) pe st0 st1)
+      (LOCAL: na_local_step p o e pe m0 m1)
+    :
+      na_step e (mk st0 m0 p o) (mk st1 m1 p o)
+  .
+
+  Variant at_step: MachineEvent.t -> t -> t -> Prop :=
+  | at_step_read
       st0 st1
-      (STEP: lang.(Language.step) ProgramEvent.silent st0 st1)
+      m0 p0 o0
+      loc val ord
+      m1 p1 o1
+      (STEP: lang.(Language.step) (ProgramEvent.read loc val ord) st0 st1)
+    :
+      at_step MachineEvent.silent (mk st0 m0 p0 o0) (mk st1 m1 p1 o1)
+  | at_step_write
+      st0 st1
+      m0 p0 o0
+      loc val ord
+      m1 p1 o1
+      (STEP: lang.(Language.step) (ProgramEvent.write loc val ord) st0 st1)
+    :
+      at_step MachineEvent.silent (mk st0 m0 p0 o0) (mk st1 m1 p1 o1)
+  | at_step_update
+      st0 st1
+      m0 p0 o0
+      loc valr valw ordr ordw
+      m1 p1 o1
+      (STEP: lang.(Language.step) (ProgramEvent.update loc valr valw ordr ordw) st0 st1)
+    :
+      at_step MachineEvent.silent (mk st0 m0 p0 o0) (mk st1 m1 p1 o1)
+  | at_step_fence
+      st0 st1
+      m0 p0 o0
+      ordr ordw
+      m1 p1 o1
+      (STEP: lang.(Language.step) (ProgramEvent.fence ordr ordw) st0 st1)
+    :
+      at_step MachineEvent.silent (mk st0 m0 p0 o0) (mk st1 m1 p1 o1)
+  | at_step_syscall
+      st0 st1
+      m0 p0 o0
+      e
+      m1 p1 o1
+      (STEP: lang.(Language.step) (ProgramEvent.syscall e) st0 st1)
+    :
+      at_step (MachineEvent.syscall e) (mk st0 m0 p0 o0) (mk st1 m1 p1 o1)
+  .
+
+  Local.program_step
+
+ProgramEvent.t
+
+  | na_step_read
+      st0 st1
+      m p o
+      loc val ord
+      (STEP: lang.(Language.step) (ProgramEvent.read loc val ord) st0 st1)
+      (ORD: Ordering.le ord Ordering.na)
+      (VAL: Perm.le Perm.full (p loc) -> fst (m loc) = val)
+    :
+      na_step MachineEvent.silent (mk st0 m p o) (mk st1 m p o)
+  | na_step_write
+      st0 st1
+      m0 p o
+      loc val ord
+      m1 e
+      (STEP: lang.(Language.step) (ProgramEvent.write loc val ord) st0 st1)
+      (ORD: Ordering.le ord Ordering.na)
+      (MEM: SeqMemory.update loc val m0 = m1)
+      (PERM: e = if Perm.le Perm.full (p loc) then MachineEvent.silent else MachineEvent.failure)
+    :
+      na_step e (mk st0 m0 p o) (mk st1 m1 p o)
+  .
+
+
+  | na_step_write_race
+      st0 st1
+      m0 p o m1
+      loc val ord
+      (STEP: lang.(Language.step) (ProgramEvent.write loc val ord) st0 st1)
+      (ORD: Ordering.le ord Ordering.na)
+      (MEM: SeqMemory.update loc val m0 = m1)
+    :
+      na_step MachineEvent.silent (mk st0 m0 p o) (mk st1 m1 p o)
+  .
+
+  | na_step_racy_read
+      st0 st1
+      loc val ord
+      (STEP: lang.(Language.step) (ProgramEvent.read loc val ord) st0 st1)
+      (ORD: Ordering.le ord Ordering.na)
       m p o
     :
       na_step (mk st0 m p o) (mk st1 m p o)
+  .
+
+
+Ordering.t
+
+
   | na_step_silent
       st0 st1
       (STEP: lang.(Language.step) ProgramEvent.silent st0 st1)
